Append unsigned native int to Bridge and adjust lemmas

Bridge.fsti
@@ -1,6 +1,7 @@
 module Bridge
 
 module I = FStar.Int
+module UI = FStar.UInt
 module L = FStar.List.Pure
 
 type result 'a 'b =
@@ -8,14 +9,22 @@ type result 'a 'b =
 | Error: e: 'b -> result 'a 'b
 
 val native_int_bits: Prims.pos
+val native_uint_bits: Prims.pos
 
 assume new type native_int
+assume new type native_uint
 
 type isize = I.int_t native_int_bits
+type usize = UI.uint_t native_uint_bits
 
 val of_int: native_int -> Tot isize
+val of_uint: native_uint -> Tot usize
 
 val to_native_int:
     #s:pos
     -> (n:I.int_t s{s <= native_int_bits})
     -> Tot (native_n:native_int{of_int native_n = n})
+val to_native_uint:
+    #s:pos
+    -> (n:UI.uint_t s{s <= native_uint_bits})
+    -> Tot (native_n:native_uint{of_uint native_n = n})
