Lemmas.String.fst
@@ -6,7 +6,7 @@ val string_of_int_return_not_empty_string: (n:int) -> Lemma (ensures S.length (s
 
 val strcat_add_length: (s1:string) -> (s2:string) -> Lemma (ensures (S.length s1) + (S.length s2) = (S.length (s1 ^ s2))) [SMTPat (s1 ^ s2)]
 
-val string_length_is_nat: (s:string) -> Lemma (S.length s >= 0)
+val string_length_is_nat: (s:string) -> Lemma (S.length s >= 0) [SMTPat (S.length s)]
 
 val empty_string_length_is_zero: (s:string) -> Lemma (requires s = "") (ensures S.length s = 0)
 
