hello-world/Hello_world.fst
@@ -1,3 +1,4 @@
 module Hello_world
 
+val hello: string
 let hello = "Hello, World!"
